LeanLinq.lean
@@ -13,5 +13,6 @@ import LeanLinq.Compiler.Expr
 import LeanLinq.Compiler.Query
 import LeanLinq.Statements
 import LeanLinq.Eval.Statements
+import LeanLinq.Freer
 import LeanLinq.Db
 import LeanLinq.Theorems
